new version of WP with no AssertionFailure
Completed WP of exetute block
WP is comuted to guarantee that Assertions never fail
Need some refactoring for theorems of executeBlock
Two cheat: related to variable substitution and EVERY vs BIGUNION

src/tools/bir_wpScript.sml
@@ -62,10 +62,13 @@ val bir_is_bool_env_exp_INTRO = prove(``
 val bir_eval_exp_subst1_env = prove(
 ``
 !ex en var ty e1.
-bir_eval_exp ex (BEnv (en |+ (var,ty,SOME (bir_eval_exp e1 (BEnv en))))) =
-bir_eval_exp (bir_exp_subst1 (BVar var ty) e1 ex) (BEnv en)
+(?r. (bir_env_lookup var (BEnv en)) = SOME (ty, r)) ==>
+(
+  bir_eval_exp ex (BEnv (en |+ (var,ty,SOME (bir_eval_exp e1 (BEnv en))))) =
+  bir_eval_exp (bir_exp_subst1 (BVar var ty) e1 ex) (BEnv en)
+)
 ``,
-REPEAT GEN_TAC >>
+REPEAT (GEN_TAC ORELSE DISCH_TAC) >>
 Induct_on `ex` >>
 ( REPEAT GEN_TAC >>
   FULL_SIMP_TAC std_ss [bir_eval_exp_def, bir_exp_subst1_REWRS]
@@ -82,10 +85,10 @@ Cases_on `var <> s` >-
 subgoal `b' <> ty` >- (
   METIS_TAC[]
 ) >>
- FULL_SIMP_TAC std_ss [] >>
+ FULL_SIMP_TAC std_ss [bir_env_lookup_def] >>
  EVAL_TAC >>
  RW_TAC std_ss [] >>
- cheat
+ CASE_TAC
 );
 
 (* ******************** *)
@@ -139,7 +142,7 @@ FULL_SIMP_TAC std_ss [bir_eval_bool_exp_INTRO, bir_mk_bool_val_true_thm]
 );
 
 (* (e /\ Q) Assume e {Q} *)
-val bir_triple_exec_strmtB_assert_thm = prove(``
+val bir_triple_exec_strmtB_assume_thm = prove(``
 ! ex post.
   (bir_is_well_typed_stmtB (BStmt_Assume ex)) ==>
   (bir_is_bool_exp post) ==>
@@ -187,90 +190,117 @@ subgoal `type_of_bir_val (bir_eval_exp ex (BEnv f)) = SOME(b)` >-
 (
  FULL_SIMP_TAC std_ss [bir_is_well_typed_stmtB_def, bir_var_type_def, type_of_bir_exp_THM_with_init_vars]
 ) >>
-FULL_SIMP_TAC std_ss [LET_DEF] >>
-RW_TAC std_ss [bir_eval_exp_subst1_env] >>
+FULL_SIMP_TAC std_ss [LET_DEF, bir_env_var_is_initialised_def] >>
+IMP_RES_TAC bir_eval_exp_subst1_env >>
+PAT_X_ASSUM ``!ex.p`` (fn thm =>
+ ASSUME_TAC (Q.SPECL [`post`, `ex`] thm)) >>
+FULL_SIMP_TAC std_ss [bir_var_name_def, bir_var_type_def] >>
+RW_TAC std_ss [] >>
+(* have atheorem that say that vars of (bir_exp_subst1 (BVar s'' b) ex post) contains *)
+(* vars of post minus s'' *)
 cheat
+);
+
+val bir_env_vars_are_initialised_observe_INSERT = prove(``
+! e ec el obf.
+(bir_env_vars_are_initialised e
+        (bir_vars_of_stmtB (BStmt_Observe ec el obf))) ==>
+(bir_env_vars_are_initialised e (bir_vars_of_exp ec))
+``,
+  REPEAT GEN_TAC >>
+  FULL_SIMP_TAC std_ss [bir_vars_of_stmtB_def, listTheory.LIST_TO_SET,
+   pred_setTheory.IMAGE_INSERT, pred_setTheory.BIGUNION_INSERT,
+   bir_env_vars_are_initialised_UNION]
 );
 
 (* {Q} Observe ex {Q} *)
 val bir_triple_exec_strmtB_observe_thm = prove(``
+! ec el obf post.
   (bir_is_well_typed_stmtB (BStmt_Observe ec el obf)) ==>
   (bir_is_bool_exp post) ==>
 bir_exec_stmtB_triple (BStmt_Observe ec el obf)
    post post
 ``,
-REWRITE_TAC [bir_exec_stmtB_triple_def] >>
-REPEAT DISCH_TAC >>
-REPEAT GEN_TAC >>
-FULL_SIMP_TAC std_ss [] >>
-REPEAT DISCH_TAC >>
-FULL_SIMP_TAC std_ss [bir_exec_stmtB_def,
-		     bir_exec_stmt_observe_def] >>
-(`bir_dest_bool_val (bir_eval_exp ec st.bst_environ) <> NONE` by cheat) >>
-Cases_on `bir_dest_bool_val (bir_eval_exp ec st.bst_environ)` >>
-FULL_SIMP_TAC std_ss [] >>
-Cases_on `x` >|
-[
- FULL_SIMP_TAC std_ss [] >>
- RW_TAC std_ss [],
- FULL_SIMP_TAC std_ss [] >>
- RW_TAC std_ss []
-]
+REWRITE_TAC [bir_exec_stmtB_triple_def, bir_pre_post_def] >>
+REPEAT (GEN_TAC ORELSE DISCH_TAC) >>
+(* Prove that the observation condition is well typed *)
+FULL_SIMP_TAC std_ss [bir_exec_stmtB_def,bir_exec_stmt_observe_def,
+  bir_is_well_typed_stmtB_def, bir_is_bool_exp_GSYM] >>
+IMP_RES_TAC bir_env_vars_are_initialised_observe_INSERT >>
+REV_FULL_SIMP_TAC std_ss [bir_is_bool_exp_env_GSYM] >>
+FULL_SIMP_TAC std_ss [bir_eval_bool_exp_INTRO, bir_mk_bool_val_inv] >>
+(* Two cases for for the observation condition *)
+Cases_on `bir_eval_bool_exp ec s.bst_environ` >>
+(FULL_SIMP_TAC std_ss [] >>
+ RW_TAC std_ss [])
 );
 
-val bir_triple_exec_strmtB_declare_thm = prove(``
-  (bir_is_well_typed_stmtB (BStmt_Declare b)) ==>
-  (bir_is_bool_exp post) ==>
-bir_exec_stmtB_triple (BStmt_Declare b)
-   post post
-``,
-cheat
-);
 
 val bir_wp_exec_stmtB_def = Define `
 (bir_wp_exec_stmtB (BStmt_Assert ex) post = (BExp_BinExp BIExp_And ex post)) /\
-(bir_wp_exec_stmtB (BStmt_Assume ex) post = 
-   (BExp_BinExp BIExp_Or (BExp_UnaryExp BIExp_Not ex) post)) /\
+(bir_wp_exec_stmtB (BStmt_Assume ex) post = (BExp_BinExp BIExp_And ex post)) /\
 (bir_wp_exec_stmtB (BStmt_Assign v ex) post = (bir_exp_subst1 v ex post)) /\
-(bir_wp_exec_stmtB (BStmt_Observe ec el obf) post = post) /\
-(bir_wp_exec_stmtB (BStmt_Declare b) post = post)
+(bir_wp_exec_stmtB (BStmt_Observe ec el obf) post = post)
+`;
+
+val bir_isnot_declare_stmt_def = Define `
+bir_isnot_declare_stmt stm = (~(?v . stm = (BStmt_Declare v)))
 `;
 
 val bir_wp_exec_stmtB_sound_thm = prove(
-``!stm post.
+``
+!stm post.
+  (bir_isnot_declare_stmt stm) ==>
   (bir_is_well_typed_stmtB stm) ==>
   (bir_is_bool_exp post) ==>
 bir_exec_stmtB_triple stm (bir_wp_exec_stmtB stm post) post
 ``,
-  REPEAT GEN_TAC >>
-  REPEAT DISCH_TAC >>
+  REPEAT (GEN_TAC ORELSE DISCH_TAC) >>
   Cases_on `stm` >>
   FULL_SIMP_TAC std_ss [bir_wp_exec_stmtB_def,
 			bir_triple_exec_strmtB_assign_thm,
 			bir_triple_exec_strmtB_assert_thm,
 			bir_triple_exec_strmtB_assume_thm,
 			bir_triple_exec_strmtB_observe_thm,
-			bir_triple_exec_strmtB_declare_thm
-		       ]
+			bir_isnot_declare_stmt_def
+		       ] >>
+  (RW_TAC std_ss [])
+);
+
+val bir_wp_exec_stmtB_bool_thm = prove(
+``
+!stm post.
+  (bir_isnot_declare_stmt stm) ==>
+  (bir_is_well_typed_stmtB stm) ==>
+  (bir_is_bool_exp post) ==>
+  (bir_is_bool_exp (bir_wp_exec_stmtB stm post))
+``,
+  REPEAT (GEN_TAC ORELSE DISCH_TAC) >>
+  Cases_on `stm` >>
+  FULL_SIMP_TAC std_ss [bir_wp_exec_stmtB_def,
+			bir_triple_exec_strmtB_assign_thm,
+			bir_triple_exec_strmtB_assert_thm,
+			bir_triple_exec_strmtB_assume_thm,
+			bir_triple_exec_strmtB_observe_thm,
+			bir_isnot_declare_stmt_def,
+			bir_is_well_typed_stmtB_def,
+			bir_is_bool_exp_GSYM,
+			bir_is_bool_exp_REWRS
+		       ] >>
+  (RW_TAC std_ss []) >>
+  (FULL_SIMP_TAC std_ss [bir_is_bool_exp_def, bir_exp_subst1_TYPE_EQ])
 );
 
 
+(* Execution of several internal statements *)
 val bir_exec_stmtsB_triple_def = Define `
 bir_exec_stmtsB_triple stmts pre post =
-!st st' fe fe' c c'.
-  (bir_is_bool_exp pre) /\
-  (bir_is_bool_exp post) /\
-(
-  (EVERY (\stmt. bir_env_vars_are_initialised st.bst_environ (bir_vars_of_stmtB stmt)) stmts) ==>
-  (bir_env_vars_are_initialised st.bst_environ (bir_vars_of_exp pre) ) ==>
-  (st.bst_status = BST_Running) ==>
-  (bir_eval_exp pre (st.bst_environ) = bir_val_true) ==>
-  (bir_exec_stmtsB stmts (fe, c, st) = (fe', c', st')) ==>
-  ((st'.bst_status = BST_AssumptionViolated) \/ (
-   (st'.bst_status = BST_Running) /\
-   (bir_eval_exp post (st'.bst_environ) = bir_val_true)
-  )))
+!s s' obs obs' c c'.
+  (EVERY (\stmt. bir_env_vars_are_initialised s.bst_environ (bir_vars_of_stmtB stmt)) stmts) ==>
+  (bir_exec_stmtsB stmts (obs, c, s) = (obs', c', s')) ==>
+  (bir_pre_post s pre s' post)
 `;
+
 
 val bir_wp_exec_stmtsB_def = Define `
 (bir_wp_exec_stmtsB [] post = post) /\
@@ -278,7 +308,25 @@ val bir_wp_exec_stmtsB_def = Define `
  bir_wp_exec_stmtB stmt (bir_wp_exec_stmtsB stmts post)
 )`;
 
+val bir_wp_exec_stmtsB_bool_thm = prove(``
+  !stmts post.
+  (EVERY bir_is_well_typed_stmtB stmts) ==>
+  (EVERY bir_isnot_declare_stmt stmts) ==>
+  (bir_is_bool_exp post) ==>
+  (bir_is_bool_exp (bir_wp_exec_stmtsB stmts post))
+``,
+  REPEAT GEN_TAC >>
+  Induct_on `stmts` >-
+  (
+   FULL_SIMP_TAC std_ss [bir_wp_exec_stmtsB_def, bir_exec_stmtsB_triple_def, bir_exec_stmtsB_def]
+  ) >>
+  REPEAT (GEN_TAC ORELSE DISCH_TAC) >>
+  FULL_SIMP_TAC std_ss [bir_wp_exec_stmtsB_def, listTheory.EVERY_DEF, bir_wp_exec_stmtB_bool_thm]
+);
+
+(* To be cleaned *)
 val exec_preserves_initialized_vars_thm = prove(``
+!r h st stmts.
 (r = bir_exec_stmtB_state (h:'a bir_stmt_basic_t) st) ==>
 (EVERY (λstmt:'a bir_stmt_basic_t.
             bir_env_vars_are_initialised st.bst_environ
@@ -287,7 +335,7 @@ val exec_preserves_initialized_vars_thm = prove(``
             bir_env_vars_are_initialised r.bst_environ
               (bir_vars_of_stmtB stmt)) stmts)
 ``,
-REPEAT DISCH_TAC >>
+REPEAT (GEN_TAC ORELSE DISCH_TAC) >>
 subgoal `!x. 
  (λstmt:'a bir_stmt_basic_t. bir_env_vars_are_initialised st.bst_environ
 	 (bir_vars_of_stmtB stmt)) x ==>
@@ -311,219 +359,181 @@ ASSUME_TAC (ISPECL [``
 REV_FULL_SIMP_TAC std_ss []
 );
 
-
-val bir_exec_stmtsB_assumption_violated_thm = prove(``
-!(q:'a option) fe c r fe' c' st'.
-(bir_exec_stmtsB stmts (OPT_CONS q fe,SUC c,r) = (fe',c',st')) ==>
-(r.bst_status <> BST_Running) ==>
-(st' = r)
-``,
-  Induct_on `stmts` >|
- [
-  REPEAT GEN_TAC >>
-  FULL_SIMP_TAC std_ss [bir_exec_stmtsB_def],
-  REPEAT GEN_TAC >>
-  FULL_SIMP_TAC std_ss [bir_exec_stmtsB_def, bir_state_is_terminated_def] >>
-  REPEAT DISCH_TAC >>
-  FULL_SIMP_TAC std_ss []
- ]);
+(* I don't think we need is anymore, since we removed assumption violated *)
+(* val bir_exec_stmtsB_assumption_violated_thm = prove(`` *)
+(* !(q:'a option) fe c r fe' c' st'. *)
+(* (bir_exec_stmtsB stmts (OPT_CONS q fe,SUC c,r) = (fe',c',st')) ==> *)
+(* (r.bst_status <> BST_Running) ==> *)
+(* (st' = r) *)
+(* ``, *)
+(*   Induct_on `stmts` >| *)
+(*  [ *)
+(*   REPEAT GEN_TAC >> *)
+(*   FULL_SIMP_TAC std_ss [bir_exec_stmtsB_def], *)
+(*   REPEAT GEN_TAC >> *)
+(*   FULL_SIMP_TAC std_ss [bir_exec_stmtsB_def, bir_state_is_terminated_def] >> *)
+(*   REPEAT DISCH_TAC >> *)
+(*   FULL_SIMP_TAC std_ss [] *)
+(*  ]); *)
   
 
 val bir_wp_exec_stmtsB_sound_thm = prove(``
   !stmts post.
   (EVERY bir_is_well_typed_stmtB stmts) ==>
+  (EVERY bir_isnot_declare_stmt stmts) ==>
   (bir_is_bool_exp post) ==>
   (bir_exec_stmtsB_triple stmts (bir_wp_exec_stmtsB stmts post) post)
 ``,
   REPEAT GEN_TAC >>
-  Induct_on `stmts` >|
-  [
-    FULL_SIMP_TAC std_ss [bir_wp_exec_stmtsB_def,
-			 bir_exec_stmtsB_triple_def,
-			 bir_exec_stmtsB_def] >>
-    RW_TAC std_ss [],
-    ALL_TAC
-  ] >>
-  GEN_TAC >>
-  REPEAT DISCH_TAC >>
-  SIMP_TAC std_ss [bir_exec_stmtsB_triple_def,
-		   Once bir_wp_exec_stmtsB_def,
-		  Once bir_exec_stmtsB_def] >>
-  REPEAT GEN_TAC >>
-  SIMP_TAC std_ss [bir_state_is_terminated_def] >>
-  Q.ABBREV_TAC `st1 = bir_exec_stmtB h st` >>
+  Induct_on `stmts` >-
+  (
+   FULL_SIMP_TAC std_ss [bir_wp_exec_stmtsB_def, bir_exec_stmtsB_triple_def, bir_exec_stmtsB_def, bir_pre_post_def]
+  ) >>
+  SIMP_TAC std_ss [bir_exec_stmtsB_triple_def, bir_pre_post_def] >>
+  REPEAT (GEN_TAC ORELSE DISCH_TAC) >>
+  FULL_SIMP_TAC std_ss [listTheory.EVERY_DEF] >>
+  FULL_SIMP_TAC std_ss [bir_exec_stmtsB_def, bir_state_is_terminated_def] >>
+  Q.ABBREV_TAC `st1 = bir_exec_stmtB h s` >>
   Cases_on `st1` >>
   FULL_SIMP_TAC std_ss [LET_DEF] >>
-
-  (* Inductive hyp *)
-  FULL_SIMP_TAC std_ss [bir_exec_stmtsB_triple_def,
-		       listTheory.EVERY_DEF] >>
-  PAT_X_ASSUM ``!st.p`` (fn thm => 
-    ASSUME_TAC (SPECL [``r:bir_state_t``, ``st':bir_state_t``,
-		      ``OPT_CONS q fe``, ``fe': 'a list``,
-		      ``SUC c``, ``c':num``] thm)) >>
-  FULL_SIMP_TAC std_ss [] >>
-
- (* wp' must be a boolean expression *)
-  Q.ABBREV_TAC `wp = (bir_wp_exec_stmtsB stmts post)` >>
   FULL_SIMP_TAC std_ss [bir_wp_exec_stmtsB_def] >>
-  ASSUME_TAC (SPECL [``h:'a bir_stmt_basic_t``, ``wp:bir_exp_t``]
-		   bir_wp_exec_stmtB_sound_thm) >>
-  REV_FULL_SIMP_TAC std_ss [bir_exec_stmtB_triple_def] >>
-  PAT_X_ASSUM ``!st.p`` (fn thm => 
-    ASSUME_TAC (SPECL [``st:bir_state_t``, ``r:bir_state_t``, ``q: 'a option``]
-		      thm)) >>
-  FULL_SIMP_TAC std_ss [] >>
-
-  (* Enable the hypothesis of wp of h *)
-  REPEAT DISCH_TAC >>
-  FULL_SIMP_TAC std_ss [] >>
-  subgoal `(bir_exec_stmtB h st = (q,r))` >|
-  [UNABBREV_ALL_TAC >> METIS_TAC [], ALL_TAC] >>
-  FULL_SIMP_TAC std_ss [] >|
-  [
-   (* Case assumption violated *)
-   ASSUME_TAC (SPECL [
-	       ``q:'a option``, ``fe: 'a list``, ``c:num``, ``r:bir_state_t``,
-	       ``fe':'a list``, ``c':num``, ``st':bir_state_t``
-     ] 
-     bir_exec_stmtsB_assumption_violated_thm) >>
-   REV_FULL_SIMP_TAC std_ss [] >>
-   RW_TAC std_ss [],
-   ALL_TAC
-  ] >>
-
-  (* case running *)
+  Q.ABBREV_TAC `wp = (bir_wp_exec_stmtsB stmts post)` >>
+  (* Handle the first step *)
+  ASSUME_TAC (Q.SPECL [`h`, `wp`] bir_wp_exec_stmtB_sound_thm) >>
+  REV_FULL_SIMP_TAC std_ss [] >>
+  IMP_RES_TAC bir_wp_exec_stmtsB_bool_thm >>
+  REV_FULL_SIMP_TAC std_ss [] >>
+  FULL_SIMP_TAC std_ss [bir_exec_stmtB_triple_def] >>
+  PAT_X_ASSUM ``!s.p`` (fn thm =>
+   ASSUME_TAC (Q.SPECL [`s`, `r`, `q`] thm)) >>
+  REV_FULL_SIMP_TAC std_ss [bir_pre_post_def] >>
+  (* Inductive hyp *)
+  FULL_SIMP_TAC std_ss [bir_exec_stmtsB_triple_def] >>
+  PAT_X_ASSUM ``!st.p`` (fn thm =>
+    ASSUME_TAC (Q.SPECL [`r`, `s'`, `OPT_CONS q obs`, `obs'`,
+		      `SUC c`, `c':num`] thm)) >>
+  REV_FULL_SIMP_TAC std_ss [] >>
   (* prove assumptions of inductive case *)
- subgoal `r = bir_exec_stmtB_state h st` >|
- [FULL_SIMP_TAC std_ss [bir_exec_stmtB_state_def],ALL_TAC] >>
-
- ASSUME_TAC exec_preserves_initialized_vars_thm >>
- REV_FULL_SIMP_TAC std_ss [] >>
- FULL_SIMP_TAC std_ss [] 
+  subgoal `r = bir_exec_stmtB_state h s` >- (
+     FULL_SIMP_TAC std_ss [bir_exec_stmtB_state_def]
+  ) >>
+  IMP_RES_TAC exec_preserves_initialized_vars_thm >>
+  FULL_SIMP_TAC std_ss [bir_pre_post_def] 
 );
 
-    
+(* Executions of the complete block, including jump *)
 val bir_exec_block_jmp_triple_def = Define(`
 bir_exec_block_jmp_triple p bl pre post l =
-!st l1 c1 st'.
-  (bir_is_bool_exp pre) /\
-  (bir_is_bool_exp post) /\
-(
-  (bir_env_vars_are_initialised st.bst_environ (bir_vars_of_block bl)) ==>
-  (bir_env_vars_are_initialised st.bst_environ (bir_vars_of_exp pre)) ==>
-  (st.bst_status = BST_Running) ==>
-  (bir_eval_exp pre (st.bst_environ) = bir_val_true) ==>
-  (bir_exec_block p bl st = (l1,c1,st')) ==>
-  ((st'.bst_status = BST_AssumptionViolated) \/ (
-   (st'.bst_status = BST_Running) /\
-   (bir_eval_exp post (st'.bst_environ) = bir_val_true) /\
-   (st'.bst_pc = bir_block_pc l)
-  )))
+!s l1 c1 s'.
+  (bir_env_vars_are_initialised s.bst_environ (bir_vars_of_block bl)) ==>
+  (bir_exec_block p bl s = (l1,c1,s')) ==>
+  (s.bst_status = BST_Running) ==>
+  (bir_is_bool_exp_env s.bst_environ pre) ==>
+  (bir_eval_exp pre (s.bst_environ) = bir_val_true) ==>
+  (
+    (s'.bst_status = BST_Running) /\
+    (bir_is_bool_exp_env s'.bst_environ post) /\
+    (bir_eval_exp post (s'.bst_environ) = bir_val_true) /\
+    (s'.bst_pc = bir_block_pc l)
+  )
 `);
+
+val bir_vars_are_initialized_block_then_every_stmts_thm = prove(``
+ (bir_env_vars_are_initialised st.bst_environ (bir_vars_of_block bl)) ==>
+ (EVERY (λstmt.
+    bir_env_vars_are_initialised st.bst_environ
+       (bir_vars_of_stmtB stmt)) bl.bb_statements)
+``,
+  FULL_SIMP_TAC std_ss [bir_vars_of_block_def, listTheory.EVERY_MEM] >>
+  REPEAT (GEN_TAC ORELSE DISCH_TAC) >>
+  cheat
+);
 
 val bir_exec_block_jmp_triple_wp_thm = prove(``
   !p bl post l.
   (bir_is_well_typed_block bl) ==>
+  (EVERY bir_isnot_declare_stmt bl.bb_statements) ==>
   (bir_is_bool_exp post) ==>
   (bl.bb_last_statement = (BStmt_Jmp (BLE_Label l))) ==>
   (MEM l (bir_labels_of_program p)) ==>
   (bir_exec_block_jmp_triple p bl 
     (bir_wp_exec_stmtsB bl.bb_statements post) post l)
 ``,
- REPEAT GEN_TAC >>
- REPEAT DISCH_TAC >>
  SIMP_TAC std_ss [bir_exec_block_jmp_triple_def] >>
- REPEAT GEN_TAC >>
- FULL_SIMP_TAC std_ss [] >>
- ASSUME_TAC (SPECL [``bl.bb_statements``,
-		   ``post:bir_exp_t``] bir_wp_exec_stmtsB_sound_thm) >>
- (REV_FULL_SIMP_TAC std_ss [bir_is_well_typed_block_def]) >>
+ REPEAT (GEN_TAC ORELSE DISCH_TAC) >>
  Q.ABBREV_TAC `wp = bir_wp_exec_stmtsB bl.bb_statements post` >>
- FULL_SIMP_TAC std_ss [bir_exec_stmtsB_triple_def] >>
- REPEAT DISCH_TAC >>
+ ASSUME_TAC (Q.SPECL [`bl.bb_statements`,`post`] bir_wp_exec_stmtsB_sound_thm) >>
+ (REV_FULL_SIMP_TAC std_ss [bir_is_well_typed_block_def, bir_exec_stmtsB_triple_def]) >>
  FULL_SIMP_TAC std_ss [bir_exec_block_def] >>
- Q.ABBREV_TAC `ns = bir_exec_stmtsB bl.bb_statements ([],0,st)` >>
+ Q.ABBREV_TAC `ns = bir_exec_stmtsB bl.bb_statements ([],0,s)` >>
  pairLib.PairCases_on `ns` >>
  FULL_SIMP_TAC std_ss [LET_DEF] >>
  PAT_X_ASSUM ``!x.p`` (fn thm =>
-   ASSUME_TAC (Q.SPECL [`st`, `ns2`, `[]:'a list`, `ns0`, `0:num`, `ns1`]
+   ASSUME_TAC (Q.SPECL [`s`, `ns2`, `[]:'a list`, `ns0`, `0:num`, `ns1`]
    thm)) >>
- REV_FULL_SIMP_TAC std_ss [] >>
- subgoal `EVERY
-         (λstmt.
-            bir_env_vars_are_initialised st.bst_environ
-              (bir_vars_of_stmtB stmt)) bl.bb_statements` >-
- (cheat) >>
- Cases_on `(ns2.bst_status = BST_AssumptionViolated)` >-
- (
-    FULL_SIMP_TAC std_ss [ bir_state_is_terminated_def] >>
-    RW_TAC std_ss [] >>
-    subgoal `(ns2 with
-  bst_pc := st.bst_pc with bpc_index := st.bst_pc.bpc_index + PRE c1).bst_status = ns2.bst_status` >-
-    (RW_TAC (srw_ss()) []) >>
-    (FULL_SIMP_TAC std_ss [])
+ REV_FULL_SIMP_TAC std_ss [bir_vars_are_initialized_block_then_every_stmts_thm] >>
+ subgoal `~(bir_state_is_terminated ns2)` >- (
+   FULL_SIMP_TAC std_ss [bir_pre_post_def, bir_state_is_terminated_def]
  ) >>
- FULL_SIMP_TAC std_ss [bir_state_is_terminated_def] >>
+ FULL_SIMP_TAC std_ss [] >>
  Q.ABBREV_TAC `st2 = (bir_exec_stmtE p (BStmt_Jmp (BLE_Label l)) ns2)` >>
  FULL_SIMP_TAC std_ss [bir_exec_stmtE_def, bir_exec_stmt_jmp_def, bir_eval_label_exp_def, bir_exec_stmt_jmp_to_label_def] >>
  REV_FULL_SIMP_TAC std_ss [Abbr `st2`] >>
  subgoal `(ns2 with bst_pc := bir_block_pc l).bst_status = ns2.bst_status` >-
  (RW_TAC (srw_ss()) []) >>
  FULL_SIMP_TAC std_ss [] >>
- subgoal `(st'.bst_status = ns2.bst_status) /\
-          (st'.bst_environ = ns2.bst_environ)` >-
+ subgoal `(s'.bst_status = ns2.bst_status) /\
+          (s'.bst_environ = ns2.bst_environ)` >-
  (RW_TAC (srw_ss()) []) >>
- (FULL_SIMP_TAC std_ss []) >>
+ (FULL_SIMP_TAC std_ss [bir_state_is_terminated_def, bir_pre_post_def]) >>
  (RW_TAC (srw_ss()) [])
-
 );
 
 
-val bir_is_bool_exp_eval_true_or_false_thm = prove(``
-! e env.
-(bir_is_bool_exp_env env e) ==>
-(((bir_dest_bool_val (bir_eval_exp e env)) = (SOME T)) \/
- ((bir_dest_bool_val (bir_eval_exp e env)) = (SOME F))
-)
-``,
-REPEAT STRIP_TAC >>
-FULL_SIMP_TAC std_ss [bir_eval_bool_exp_INTRO, bir_mk_bool_val_def, bool2b_def,
-bir_dest_bool_val_def]
-);
+(* val bir_is_bool_exp_eval_true_or_false_thm = prove(`` *)
+(* ! e env. *)
+(* (bir_is_bool_exp_env env e) ==> *)
+(* (((bir_dest_bool_val (bir_eval_exp e env)) = (SOME T)) \/ *)
+(*  ((bir_dest_bool_val (bir_eval_exp e env)) = (SOME F)) *)
+(* ) *)
+(* ``, *)
+(* REPEAT STRIP_TAC >> *)
+(* FULL_SIMP_TAC std_ss [bir_eval_bool_exp_INTRO, bir_mk_bool_val_def, bool2b_def, *)
+(* bir_dest_bool_val_def] *)
+(* ); *)
 
-val bir_exec_block_cjmp_triple_def = Define(`
+val bir_exec_block_cjmp_triple_def = Define `
 bir_exec_block_cjmp_triple p bl pre post1 l1 post2 l2 =
-!st l' c1 st'.
-  (bir_is_bool_exp pre) /\
-  (bir_is_bool_exp post1) /\
-  (bir_is_bool_exp post2) /\
-(
-  (bir_env_vars_are_initialised st.bst_environ (bir_vars_of_block bl)) ==>
-  (bir_env_vars_are_initialised st.bst_environ (bir_vars_of_exp pre)) ==>
-  (st.bst_status = BST_Running) ==>
-  (bir_eval_exp pre (st.bst_environ) = bir_val_true) ==>
-  (bir_exec_block p bl st = (l',c1,st')) ==>
-  ((st'.bst_status = BST_AssumptionViolated) \/ (
-   (st'.bst_status = BST_Running) /\ ((
-     (bir_eval_exp post1 (st'.bst_environ) = bir_val_true) /\
-     (st'.bst_pc = bir_block_pc l1))
-     \/ (
-     (bir_eval_exp post2 (st'.bst_environ) = bir_val_true) /\
-     (st'.bst_pc = bir_block_pc l2)))
-  )))
-`);
+!s obs' c1 s'.
+  (bir_env_vars_are_initialised s.bst_environ (bir_vars_of_block bl)) ==>
+  (bir_exec_block p bl s = (obs',c1,s')) ==>
+  (s.bst_status = BST_Running) ==>
+  (bir_is_bool_exp_env s.bst_environ pre) ==>
+  (bir_eval_exp pre (s.bst_environ) = bir_val_true) ==>
+  (
+    (s'.bst_status = BST_Running) /\
+    ((
+      (bir_is_bool_exp_env s'.bst_environ post1) /\
+      (bir_eval_exp post1 (s'.bst_environ) = bir_val_true) /\
+      (s'.bst_pc = bir_block_pc l1)
+    ) \/ (
+      (bir_is_bool_exp_env s'.bst_environ post2) /\
+      (bir_eval_exp post2 (s'.bst_environ) = bir_val_true) /\
+      (s'.bst_pc = bir_block_pc l2)
+    ))
+  )
+`;
 
 
 val bir_exec_block_cjmp_triple_wp_thm = prove(``
-  !p bl post1 l1 post2 l2.
+  !p bl e post1 l1 post2 l2.
   (bir_is_well_typed_block bl) ==>
+  (EVERY bir_isnot_declare_stmt bl.bb_statements) ==>
   (bir_is_bool_exp post1) ==>
   (bir_is_bool_exp post2) ==>
   (bl.bb_last_statement = (BStmt_CJmp e (BLE_Label l1) (BLE_Label l2))) ==>
   (MEM l1 (bir_labels_of_program p)) ==>
   (MEM l2 (bir_labels_of_program p)) ==>
-
   (bir_exec_block_cjmp_triple p bl 
     (bir_wp_exec_stmtsB bl.bb_statements  (
     (BExp_BinExp BIExp_And 
@@ -533,325 +543,73 @@ val bir_exec_block_cjmp_triple_wp_thm = prove(``
     ))
     post1 l1 post2 l2)
 ``,
- REPEAT GEN_TAC >>
- REPEAT DISCH_TAC >>
  SIMP_TAC std_ss [bir_exec_block_cjmp_triple_def] >>
- REPEAT GEN_TAC >>
- FULL_SIMP_TAC std_ss [] >>
-
+ REPEAT (GEN_TAC ORELSE DISCH_TAC) >>
  Q.ABBREV_TAC `q1 = (BExp_BinExp BIExp_Or (BExp_UnaryExp BIExp_Not e) post1)` >> 
  Q.ABBREV_TAC `q2 = (BExp_BinExp BIExp_Or e post2)` >>
  Q.ABBREV_TAC `post_stmts = (BExp_BinExp BIExp_And q1 q2)` >> 
-
- ASSUME_TAC (SPECL [``bl.bb_statements``,
-		   ``post_stmts:bir_exp_t``] bir_wp_exec_stmtsB_sound_thm) >>
- (REV_FULL_SIMP_TAC std_ss [bir_is_well_typed_block_def]) >>
-
+ Q.ABBREV_TAC `wp = bir_wp_exec_stmtsB bl.bb_statements post_stmts` >>
+ (* We use the fact that the WP of internal statements is sound *)
+ ASSUME_TAC (Q.SPECL [`bl.bb_statements`,`post_stmts`] bir_wp_exec_stmtsB_sound_thm) >>
+ (REV_FULL_SIMP_TAC std_ss [bir_is_well_typed_block_def, bir_exec_stmtsB_triple_def]) >>
  subgoal `bir_is_bool_exp post_stmts` >-
  (
-  FULL_SIMP_TAC std_ss [Abbr `q1`, Abbr `q2`, Abbr `post_stmts`, bir_is_bool_exp_REWRS,
-		 bir_is_well_typed_stmtE_def,
-		 BType_Bool_def,
-		 GSYM bir_is_bool_exp_def
-		]
+  FULL_SIMP_TAC std_ss [Abbr `q1`, Abbr `q2`, Abbr `post_stmts`,
+    bir_is_bool_exp_REWRS, bir_is_well_typed_stmtE_def, BType_Bool_def,
+    GSYM bir_is_bool_exp_def]
  ) >>
- FULL_SIMP_TAC std_ss [bir_exec_stmtsB_triple_def] >>
-
+ (* Open the definition of exec block *)
  FULL_SIMP_TAC std_ss [bir_exec_block_def] >>
- Q.ABBREV_TAC `ns = bir_exec_stmtsB bl.bb_statements ([],0,st)` >>
+ Q.ABBREV_TAC `ns = bir_exec_stmtsB bl.bb_statements ([],0,s)` >>
  pairLib.PairCases_on `ns` >>
  FULL_SIMP_TAC std_ss [LET_DEF] >>
-
  PAT_X_ASSUM ``!x.p`` (fn thm =>
-   ASSUME_TAC (Q.SPECL [`st`, `ns2`, `[]:'a list`, `ns0`, `0:num`, `ns1`]
+   ASSUME_TAC (Q.SPECL [`s`, `ns2`, `[]:'a list`, `ns0`, `0:num`, `ns1`]
    thm)) >>
- FULL_SIMP_TAC std_ss [] >>
- REPEAT DISCH_TAC >>
-
- subgoal `EVERY
-         (λstmt.
-            bir_env_vars_are_initialised st.bst_environ
-              (bir_vars_of_stmtB stmt)) bl.bb_statements` >-
- (cheat) >>
- (FULL_SIMP_TAC std_ss []) >>
-
- Cases_on `(ns2.bst_status = BST_AssumptionViolated)` >-
- (
-    FULL_SIMP_TAC std_ss [ bir_state_is_terminated_def] >>
-    RW_TAC std_ss [] >>
-    subgoal `(ns2 with
-  bst_pc := st.bst_pc with bpc_index := st.bst_pc.bpc_index + PRE c1).bst_status = ns2.bst_status` >-
-    (RW_TAC (srw_ss()) []) >>
-    (FULL_SIMP_TAC std_ss [])
+ REV_FULL_SIMP_TAC std_ss [bir_vars_are_initialized_block_then_every_stmts_thm] >>
+ subgoal `~(bir_state_is_terminated ns2)` >- (
+   FULL_SIMP_TAC std_ss [bir_pre_post_def, bir_state_is_terminated_def]
  ) >>
- FULL_SIMP_TAC std_ss [bir_state_is_terminated_def] >>
- REV_FULL_SIMP_TAC std_ss [] >>
+ FULL_SIMP_TAC std_ss [] >>
  Q.ABBREV_TAC `st2 = (bir_exec_stmtE p (BStmt_CJmp e (BLE_Label l1) (BLE_Label l2)) ns2)` >>
  FULL_SIMP_TAC std_ss [bir_exec_stmtE_def, bir_exec_stmt_cjmp_def] >>
  (* to proove that is_bool e *)
- FULL_SIMP_TAC std_ss [bir_is_well_typed_stmtE_def,
-		      BType_Bool_def,
-		     GSYM bir_is_bool_exp_def] >>
- subgoal `bir_env_vars_are_initialised st.bst_environ
-         (bir_vars_of_exp e)` >-
- (cheat) >>
- REV_FULL_SIMP_TAC std_ss [bir_is_bool_exp_env_GSYM] >>
- Cases_on `(bir_dest_bool_val (bir_eval_exp e ns2.bst_environ) = SOME T)` >-
+ subgoal `bir_is_bool_exp_env ns2.bst_environ e` >-
  (
-   FULL_SIMP_TAC std_ss [bir_exec_stmt_jmp_def,
-			bir_eval_label_exp_def,
-			bir_exec_stmt_jmp_to_label_def] >>
-   REV_FULL_SIMP_TAC std_ss [Abbr `st2`] >>
-   subgoal `(ns2 with bst_pc := bir_block_pc l1).bst_status = ns2.bst_status` >-
-   (RW_TAC (srw_ss()) []) >>
-   FULL_SIMP_TAC std_ss [] >>
-   REV_FULL_SIMP_TAC std_ss [] >>
-   subgoal `(st'.bst_environ = ns2.bst_environ)` >-
-   (RW_TAC (srw_ss()) []) >>
-   (FULL_SIMP_TAC std_ss []) >>
-   FULL_SIMP_TAC std_ss [Abbr `post_stmts`, Abbr `q1`, Abbr `q2`] >> 
-   (* general proof that var_initialized_block /\ var_initialized_wp => var_initialided post *)
-   subgoal `bir_is_bool_exp_env ns2.bst_environ
-            (BExp_BinExp BIExp_And
-               (BExp_BinExp BIExp_Or (BExp_UnaryExp BIExp_Not e) post1)
-               (BExp_BinExp BIExp_Or e post2))` >-
-   (cheat) >>
-   FULL_SIMP_TAC std_ss [bir_eval_bool_exp_INTRO] >>
-   FULL_SIMP_TAC std_ss [Once (GEN ``env:bir_var_environment_t`` bir_is_bool_exp_env_REWRS)] >>
-   FULL_SIMP_TAC std_ss [Once bir_eval_bool_exp_BExp_BinExp_REWRS] >>
-   FULL_SIMP_TAC std_ss [Once (GEN ``env:bir_var_environment_t`` bir_is_bool_exp_env_REWRS)] >>
-   FULL_SIMP_TAC std_ss [Once bir_eval_bool_exp_BExp_BinExp_REWRS] >>
-   FULL_SIMP_TAC std_ss [Once (GEN ``env:bir_var_environment_t`` bir_is_bool_exp_env_REWRS)] >>
-   FULL_SIMP_TAC std_ss [Once bir_eval_bool_exp_BExp_UnaryExp_REWRS] >>
-   
-   subgoal `bir_eval_bool_exp e ns2.bst_environ` >- (cheat) >>
-   FULL_SIMP_TAC std_ss [bir_mk_bool_val_true_thm] >>
-
-   ASM_SIMP_TAC std_ss [bir_eval_bool_exp_INTRO] >>
-   FULL_SIMP_TAC std_ss [bir_mk_bool_val_true_thm] >>
-   (* Proved that post1 hold *)
-   RW_TAC std_ss []
+  FULL_SIMP_TAC std_ss [bir_pre_post_def] >>
+  REV_FULL_SIMP_TAC std_ss [Abbr `post_stmts`, Abbr `q1`, Abbr `q2`] >>
+  IMP_RES_TAC bir_is_bool_env_exp_INTRO >>
+  IMP_RES_TAC bir_is_bool_env_exp_INTRO
  ) >>
- (* bir_is_bool_exp_eval_true_or_false_thm *)
- cheat
+ FULL_SIMP_TAC std_ss [bir_eval_bool_exp_INTRO, bir_mk_bool_val_inv] >>
+ REV_FULL_SIMP_TAC std_ss [bir_pre_post_def] >>
+ (* Better to have a theorem *)
+ (* Proves that since eval_bool (q1 /\ q2) then eval_bool q1 /\ eval_bool q2 *)
+ FULL_SIMP_TAC std_ss [Abbr `post_stmts`] >>
+ IMP_RES_TAC bir_is_bool_env_exp_INTRO >>
+ FULL_SIMP_TAC std_ss [bir_eval_bool_exp_INTRO, bir_mk_bool_val_true_thm,
+    bir_eval_bool_exp_BExp_BinExp_REWRS] >>
+ Cases_on `bir_eval_bool_exp e ns2.bst_environ` >-
+ (
+    FULL_SIMP_TAC std_ss [bir_exec_stmt_jmp_def, bir_eval_label_exp_def, bir_exec_stmt_jmp_to_label_def] >>
+    REV_FULL_SIMP_TAC std_ss [Abbr `st2`, bir_state_is_terminated_def] >>
+    RW_TAC std_ss [] >>
+    FULL_SIMP_TAC std_ss [Abbr `q1`] >>
+    IMP_RES_TAC bir_is_bool_env_exp_INTRO >>
+    subgoal `~(bir_eval_bool_exp (BExp_UnaryExp BIExp_Not e) ns2.bst_environ) ` >-
+    (
+     FULL_SIMP_TAC std_ss [bir_eval_bool_exp_BExp_UnaryExp_REWRS]
+    ) >>
+    FULL_SIMP_TAC std_ss [bir_eval_bool_exp_BExp_BinExp_REWRS, bir_eval_bool_exp_INTRO, bir_mk_bool_val_true_thm]
+ ) >>
+ (* second case when e does not hold *)
+ FULL_SIMP_TAC std_ss [bir_exec_stmt_jmp_def, bir_eval_label_exp_def, bir_exec_stmt_jmp_to_label_def] >>
+ REV_FULL_SIMP_TAC std_ss [Abbr `st2`, bir_state_is_terminated_def] >>
+ RW_TAC std_ss [] >>
+ FULL_SIMP_TAC std_ss [Abbr `q2`] >>
+ IMP_RES_TAC bir_is_bool_env_exp_INTRO >>
+ FULL_SIMP_TAC std_ss [bir_eval_bool_exp_BExp_BinExp_REWRS, bir_eval_bool_exp_INTRO, bir_mk_bool_val_true_thm]
 );
 
 
 val _ = export_theory();
-
-
-
-
-
-
-
-
-
-
-
-
-
-
-
-(*
-
-``
-(bir_env_vars_are_initialised st.bst_environ
- (bir_vars_of_program p)) ==>
-((bir_wp_exec_stmtsB bl.bb_statements post) = wp) ==>
-(bir_env_vars_are_initialised st.bst_environ
-         (bir_vars_of_exp wp)) ==>
-(st.bst_status = BST_Running) ==>
-(bir_eval_exp wp st.bst_environ = bir_val_true) ==>
-(bir_is_well_typed_program p) ==>
-(bir_is_bool_exp post) ==>
-(bir_get_current_block p st.bst_pc = SOME bl) ==>
-(bl.bb_last_statement = (BStmt_Jmp (BLE_Label l))) ==>
-(l ∈ ls) ==>
-(? l1 c1 n st1. (bir_exec_to_labels ls p st = (BER_Ended l1 c1 n st1)) /\
-  ((st'.bst_status = BST_AssumptionViolated) \/ 
-   (bir_eval_exp post (st'.bst_environ) = bir_val_true)
-  )
-)
-``
-REPEAT DISCH_TAC >>
-ASSUME_TAC (SPECL [``ls:bir_label_t -> bool``, ``p:'a bir_program_t``,
-		   ``st:bir_state_t``, ``bl:'a bir_block_t``]
-	    bir_exec_to_labels_block
-) >>
-Q.ABBREV_TAC `e' = (bir_exec_to_labels ls p st =
-       (let (l1,c1,st1) = bir_exec_block p bl st
-        in
-          if
-            0 < c1 ∧
-            bir_state_COUNT_PC
-              (F,(λpc. (pc.bpc_index = 0) ∧ pc.bpc_label ∈ ls)) st1
-          then
-            BER_Ended l1 c1 1 st1
-          else
-            case bir_exec_to_labels ls p st1 of
-              BER_Ended l2 c2 c2' st2 =>
-                BER_Ended (l1 ++ l2) (c1 + c2) c2' st2
-            | BER_Looping ll2 =>
-                BER_Looping (LAPPEND (fromList l1) ll2)))` >>
-REV_FULL_SIMP_TAC std_ss [] >>
-Q.ABBREV_TAC `r = bir_exec_block p bl st` >>
-pairLib.PairCases_on `r` >>
-FULL_SIMP_TAC std_ss [LET_DEF] >>
-FULL_SIMP_TAC std_ss [bir_exec_block_def] >>
-
-(* This is for the list of internal statements *)
-ASSUME_TAC (SPECL [``bl.bb_statements : 'a bir_stmt_basic_t list``,
-		   ``post:bir_exp_t``] bir_wp_exec_stmtsB_sound_thm) >>
-FULL_SIMP_TAC std_ss [bir_is_well_typed_program_def] >>
-subgoal `bir_is_well_typed_block bl` >| [cheat, ALL_TAC] >>
-FULL_SIMP_TAC std_ss [bir_is_well_typed_block_def] >>
-
-REV_FULL_SIMP_TAC std_ss [bir_exec_stmtsB_triple_def] >>
-PAT_X_ASSUM ``!st:bir_state_t.p`` (fn thm =>
-  ASSUME_TAC (SPECL [``st:bir_state_t``, ``st':bir_state_t``,
-		     ``[]: 'a list``, ``fe':'a list``,
-		     ``0:num``, ``c':num``] thm)) >>
-FULL_SIMP_TAC std_ss [] >>
-
-
-
-bir_program_blocksTheory.bir_exec_to_labels_block;
-
-
-  (bir_is_bool_exp pre) /\
-   /\
-(
-  (EVERY (\stmt. bir_env_vars_are_initialised st.bst_environ (bir_vars_of_stmtB stmt)) stmts) ==>
-  (bir_env_vars_are_initialised st.bst_environ (bir_vars_of_exp pre) ) ==>
-  (st.bst_status = BST_Running) ==>
-  (bir_eval_exp pre (st.bst_environ) = bir_val_true) ==>
-  (bir_exec_stmtsB stmts (fe, c, st) = (fe', c', st')) ==>
-  ((st'.bst_status = BST_AssumptionViolated) \/ (
-   (st'.bst_status = BST_Running) /\
-   (bir_eval_exp post (st'.bst_environ) = bir_val_true)
-  )))
-
-
-*)
-(* val bir_exec_to_labels_triple_def = Define ` *)
-(* bir_exec_to_labels_triple ls lstart p pre post = *)
-(* !bs. *)
-(*   (bir_eval_exp pre (bs.bst_environ) = bir_val_true) ==> *)
-(*   (bs.bst_pc = <| bpc_label := lstart; bpc_index:= 0 |>) ==> *)
-(*   ?lo c_st c_addr_labels bs'. *)
-(*   (bir_exec_to_labels ls p bs = BER_Ended lo c_st c_addr_labels bs') /\ *)
-(*   (~(bs'.bst_status = BST_AssertionViolated)) /\ *)
-(*   ((bs'.bst_status = BST_AssumptionViolated) \/ *)
-(*    (bir_eval_exp post (bs'.bst_environ) = bir_val_true) *)
-(*   ) *)
-(* `; *)
-
-(* val bir_exec_block_triple_def = Define ` *)
-(* bir_exec_block_triple lstart p pre post = *)
-(* !bs bl. *)
-(*   (bir_eval_exp pre (bs.bst_environ) = bir_val_true) ==> *)
-(*   (bs.bst_pc = <| bpc_label := lstart; bpc_index:= 0 |>) ==> *)
-(*   (bir_get_current_block p bs.bst_pc = SOME bl) ==> *)
-(*   ?l1,c1,bs'. *)
-(*   (bir_exec_block p bl bs = (l1,c1,bs')) /\ *)
-(*   (~(bs'.bst_status = BST_AssertionViolated)) /\ *)
-(*   ((bs'.bst_status = BST_AssumptionViolated) \/ *)
-(*    (bir_eval_exp post (bs'.bst_environ) = bir_val_true) *)
-(*   ) *)
-(* `; *)
-
-
-
-(* val bir_exec_stmtE_triple_def = Define ` *)
-(* bir_exec_stmtE_triple p stmt pre post = *)
-(* !st st'. *)
-(*   (bir_env_vars_are_initialised st.bst_environ (bir_vars_of_stmtE stmt) ) ==> *)
-(*   (st.bst_status = BST_Running) ==> *)
-(*   (bir_eval_exp pre (st.bst_environ) = bir_val_true) ==> *)
-(*   (bir_exec_stmtE p stmt st = st') ==> *)
-(*   (~(st'.bst_status = BST_AssertionViolated)) /\ *)
-(*   ((st'.bst_status = BST_AssumptionViolated) \/ *)
-(*    (bir_eval_exp post (st'.bst_environ) = bir_val_true) *)
-(*   ) *)
-(* `; *)
-
-(* prove(`` *)
-(*   bir_is_well_typed_stmtE c ==> *)
-(*   bir_exec_stmtE_triple p (BStmt_Halt ex) post post *)
-(* ``, *)
-(* REWRITE_TAC [bir_exec_stmtE_triple_def] >> *)
-(* DISCH_TAC >> (REPEAT GEN_TAC) >> *)
-(* REPEAT DISCH_TAC >> *)
-(* FULL_SIMP_TAC std_ss [bir_exec_stmtE_def,bir_exec_stmt_halt_def] >> *)
-(* (RW_TAC std_ss []) *)
-(* ); *)
-
-
-
-(* val bir_wp_exec_stmtE_def = Define ` *)
-(* (bir_wp_exec_stmtE p (BStmt_Halt ex) post = post) /\ *)
-(* (bir_wp_exec_stmtE p (BStmt_Jmp l) post = post) /\ *)
-(* (bir_wp_exec_stmtE p (BStmt_CJmp b b0 b1) post = post) *)
-(* `; *)
-
-(* (* Must be cleaned, but htis is the basic idea *) *)
-(* prove (`` *)
-(* bir_is_well_typed_stmtE c ==> *)
-(* bir_exec_stmtE_triple p c *)
-(*   (bir_wp_exec_stmtE p c post) post *)
-(* ``, *)
-(* REPEAT DISCH_TAC >> *)
-(* REWRITE_TAC [bir_exec_stmtE_triple_def] >> *)
-(* REPEAT GEN_TAC >> *)
-(* REPEAT DISCH_TAC >> *)
-(* Cases_on `c`  *)
-(* >| *)
-(* [ *)
-(*  FULL_SIMP_TAC std_ss [bir_exec_stmtE_def, *)
-(* 		       bir_exec_stmt_jmp_def, *)
-(* 		       bir_is_well_typed_stmtE_def, *)
-(* 		       bir_vars_of_stmtE_def, *)
-(* 		       bir_wp_exec_stmtE_def *)
-(* 		      ] >> *)
-(*  ASSUME_TAC (SPECL [``b:bir_label_exp_t``, ``st.bst_environ``] *)
-(* 	    	   bir_eval_label_exp_NEQ_NONE_WF_INITIALISED *)
-(* 	    ) >> *)
-(*  REV_FULL_SIMP_TAC std_ss [] >> *)
-(*  Cases_on `bir_eval_label_exp b st.bst_environ` >> *)
-(*  (FULL_SIMP_TAC std_ss []) >> *)
-(*  (FULL_SIMP_TAC std_ss [bir_exec_stmt_jmp_to_label_def]) >> *)
-(*  (RW_TAC std_ss []), *)
-
-(*  FULL_SIMP_TAC std_ss [bir_exec_stmtE_def, *)
-(* 		       bir_exec_stmt_cjmp_def, *)
-(* 		       bir_exec_stmt_jmp_def, *)
-(* 		       bir_is_well_typed_stmtE_def, *)
-(* 		       bir_vars_of_stmtE_def, *)
-(* 		       bir_wp_exec_stmtE_def *)
-(* 		      ] >> *)
-(*  ASSUME_TAC (SPECL [``b0:bir_label_exp_t``, ``st.bst_environ``] *)
-(* 	    	   bir_eval_label_exp_NEQ_NONE_WF_INITIALISED *)
-(* 	    ) >> *)
-(*  ASSUME_TAC (SPECL [``b1:bir_label_exp_t``, ``st.bst_environ``] *)
-(* 	    	   bir_eval_label_exp_NEQ_NONE_WF_INITIALISED *)
-(* 	    ) >> *)
-(*  REV_FULL_SIMP_TAC std_ss [bir_env_vars_are_initialised_UNION] >> *)
-(*  Cases_on `bir_eval_label_exp b0 st.bst_environ` >> *)
-(*  (FULL_SIMP_TAC std_ss []) >> *)
-(*  Cases_on `bir_eval_label_exp b1 st.bst_environ` >> *)
-(*  (FULL_SIMP_TAC std_ss []) >> *)
-(*  (`bir_dest_bool_val (bir_eval_exp b st.bst_environ) <> NONE` by cheat) >> *)
-(*  (FULL_SIMP_TAC std_ss [bir_exec_stmt_jmp_to_label_def]) >> *)
-(*  Cases_on `(bir_dest_bool_val (bir_eval_exp b st.bst_environ))` >> *)
-(*  (FULL_SIMP_TAC std_ss []) >> *)
-(*  (RW_TAC std_ss []), *)
-
-(*  FULL_SIMP_TAC std_ss [bir_exec_stmtE_def, *)
-(* 		       bir_exec_stmt_halt_def, *)
-(* 		       bir_wp_exec_stmtE_def *)
-(* 		      ] >> *)
-(*  (RW_TAC std_ss []) *)
-(* ] *)
-
-(* ); *)
